Derived_Terms.v
@@ -1,42 +1,24 @@
 (**************************************************************************)
-(*  This is part of STATES, it is distributed under the terms of the      *)
-(*         GNU Lesser General Public License version 3                    *)
-(*              (see file LICENSE for more details)                       *)
+(*  This is part of IMP-STATES, it is distributed under the terms of the  *)
+(*              GNU Lesser General Public License version 3               *)
+(*                  (see file LICENSE for more details)                   *)
 (*                                                                        *)
-(*       Copyright 2013: Jean-Guillaume Dumas, Dominique Duval            *)
+(*       Copyright 2014: Jean-Guillaume Dumas, Dominique Duval            *)
 (*			 Burak Ekici, Damien Pous.                        *)
 (**************************************************************************)
 
 Require Import Relations Morphisms.
 Require Import Program.
-Require Memory Terms Decorations Axioms.
+Require Memory Terms Decorations.
 Set Implicit Arguments.
 
 Module Make(Import M: Memory.T).
-  Module Export Derived_TermsExp := Axioms.Make(M). 
+  Module Export Derived_TermsExp := Decorations.Make(M). 
 
- Definition prod_forget {X Y}: term unit (X/*/Y) := (@forget (X/*/Y)).
- Definition iso {X}: term (X/*/unit) X := pair (@id X) (@forget X). 
- Definition inv_pi1 {X}: term (X/*/unit) X := pair (@id X) (@forget X). 
- Definition permut {X Y}: term (X/*/Y) (Y/*/X) := pair (@pi2 Y X) (@pi1 Y X).
- 
- Definition perm_pair {X Y Z} (f: term Y X) (g: term Z X): term (Y/*/Z) X
- := permut o pair g f.
- Definition prod {X Y X' Y'} (f: term X X') (g: term Y Y'): term (X/*/Y) (X'/*/Y')
- := pair (f o (@pi1 X' Y')) (g o (@pi2 X' Y')).
- Definition perm_prod {X Y X' Y'} (f: term X X') (g: term Y Y'): term (X/*/Y) (X'/*/Y')
- := perm_pair (f o (@pi1 X' Y')) (g o (@pi2 X' Y')).
+ (*For states*)
 
- Check boolT.
-
- (*For exceptions*)
-
- Definition throw (X: Type) (t2: EName) := (@empty X) o tag t2.
- Definition exc_iso {X}: term (X/+/empty_set) X := (@copi1 X empty_set).
- Definition TRY {X Y} (f: term Y X) (k: term Y empty_set)
-  := (copair id k) o exc_iso o f.
- Definition TRY_CATCH (X Y: Type) (t: EName) (f: term Y X) (g: term Y unit)
-  := downcast((copair (@id Y) (g o (untag t))) o exc_iso o f).
+ Definition ttrue:  term boolT unit := (@copi1 unit unit).
+ Definition ffalse: term boolT unit := (@copi2 unit unit). 
 
  Lemma is_ttrue: is pure (@copi1 unit unit).
  Proof. auto. Qed.
@@ -44,53 +26,4 @@ Module Make(Import M: Memory.T).
  Lemma is_ffalse: is pure (@copi2 unit unit).
  Proof. auto. Qed.
  
- Lemma is_prod_forget X Y: is pure (@prod_forget X Y).
- Proof.
-     unfold prod_forget. apply is_forget.
- Qed.
-
- Lemma is_inv_pi1 X: is pure (@inv_pi1 X).
- Proof.
-     unfold inv_pi1. apply is_pair.
-     apply is_id. apply is_forget.
- Qed.
- 
- Lemma is_permut X Y: is pure (@permut X Y).
- Proof.
-     unfold permut. apply is_pair. 
-     apply is_pi2. apply is_pi1.
- Qed.
-
- Lemma is_perm_pair: forall k X Y Z (f: term Y X) (g: term Z X),
- is k f -> is k g -> is k (perm_pair f g).
- Proof.
-     intros. unfold perm_pair. apply is_comp.
-     induction k. apply is_permut. apply is_pure_ro.
-     apply is_permut. apply is_ro_rw. apply is_pure_ro.
-     apply is_permut. apply is_pair.
-     assumption. assumption.
- Qed.
-
- Lemma is_prod: forall k X' X Y' Y (f: term X X') (g: term Y Y'), 
- is k f -> is k g -> is k (prod f g).
- Proof.
-     intros. apply is_pair. apply is_comp. assumption.
-     induction k. apply is_pi1. apply is_pure_ro. apply is_pi1. 
-     apply is_ro_rw. apply is_pure_ro. apply is_pi1.
-     apply is_comp. assumption.
-     induction k. apply is_pi2. apply is_pure_ro. apply is_pi2. 
-     apply is_ro_rw. apply is_pure_ro. apply is_pi2.
- Qed. 
-
- Lemma is_perm_prod: forall k X' X Y' Y (f: term X X') (g: term Y Y'), 
- is k f -> is k g -> is k (perm_pair (f o (@pi1 X' Y')) (g o (@pi2 X' Y'))).
- Proof.
-     intros. apply is_perm_pair. apply is_comp. assumption.
-     induction k. apply is_pi1. apply is_pure_ro. apply is_pi1. 
-     apply is_ro_rw. apply is_pure_ro. apply is_pi1.
-     apply is_comp. assumption.
-     induction k. apply is_pi2. apply is_pure_ro. apply is_pi2. 
-     apply is_ro_rw. apply is_pure_ro. apply is_pi2.
- Qed.
-
 End Make.
