IMP_Proofs.v
@@ -1,124 +1,22 @@
 (**************************************************************************)
-(*  This is part of STATES, it is distributed under the terms of the      *)
-(*         GNU Lesser General Public License version 3                    *)
-(*              (see file LICENSE for more details)                       *)
+(*  This is part of IMP-STATES, it is distributed under the terms of the  *)
+(*              GNU Lesser General Public License version 3               *)
+(*                  (see file LICENSE for more details)                   *)
 (*                                                                        *)
-(*       Copyright 2013: Jean-Guillaume Dumas, Dominique Duval            *)
+(*       Copyright 2014: Jean-Guillaume Dumas, Dominique Duval            *)
 (*			 Burak Ekici, Damien Pous.                        *)
 (**************************************************************************)
 
 Require Import Relations Morphisms.
 Require Import Program.
-Require Memory Terms Decorations Axioms Derived_Terms Derived_Pairs
-Derived_Products Derived_Rules Proofs.
+Require Memory Terms Decorations Derived_Terms Axioms
+Derived_Rules IMP_to_COQ.
 Set Implicit Arguments.
 Require Import ZArith.
 Open Scope Z_scope.
 
 Module Make(Import M: Memory.T).
-  Module Export ConversionExp := Proofs.Make(M).
-
- Inductive ArithExp : Type :=
-    | const    : Z -> ArithExp
-    | loc      : Loc -> ArithExp
-    | add      : ArithExp -> ArithExp -> ArithExp
-    | multiply : ArithExp -> ArithExp -> ArithExp.
-
- Fixpoint defArithExp (a: ArithExp) : term Z unit :=
-  match a with
-    | const n        => (@constant Z n)
-    | loc x          => (lookup x)
-    | add t1 t2      => plus o (pair (defArithExp t1) (defArithExp t2))
-    | multiply t3 t4 => mult o (pair (defArithExp t3) (defArithExp t4))
-  end.
-
- Inductive BoolExp : Type :=
-    | constT  : term boolT unit -> BoolExp
-    | constF  : term boolT unit -> BoolExp
-    | gtT     : ArithExp -> ArithExp -> BoolExp
-    | geT     : ArithExp -> ArithExp -> BoolExp
-    | ltT     : ArithExp -> ArithExp -> BoolExp
-    | leT     : ArithExp -> ArithExp -> BoolExp
-    | eqT     : ArithExp -> ArithExp -> BoolExp
-    | andT    : BoolExp -> BoolExp -> BoolExp
-    | orT     : BoolExp -> BoolExp -> BoolExp.
-
- Fixpoint defBoolExp (b: BoolExp) : term boolT unit :=
-  match b with
-    | constT ttrue  => ttrue
-    | constF ffalse => ffalse
-    | gtT a1 a2     => (gt o (pair (defArithExp a1) (defArithExp a2)))
-    | geT a1 a2     => (ge o (pair (defArithExp a1) (defArithExp a2)))
-    | ltT a1 a2     => (lt o (pair (defArithExp a1) (defArithExp a2)))
-    | leT a1 a2     => (le o (pair (defArithExp a1) (defArithExp a2)))
-    | eqT a1 a2     => (eq o (pair (defArithExp a1) (defArithExp a2)))
-    | andT b1 b2    => (andB o (pair (defBoolExp b1) (defBoolExp b2)))
-    | orT b3 b4     => (orB o (pair (defBoolExp b3) (defBoolExp b4)))
-  end.
-
- Inductive Command : Type :=
-    | skip       : Command
-    | sequence   : Command -> Command -> Command
-    | assign     : Loc -> ArithExp -> Command 
-    | ifthenelse : BoolExp -> Command -> Command -> Command
-    | loops      : BoolExp -> Command -> Command
-    | throwexc   : EName -> Command
-    | trycatch   : EName -> Command -> Command -> Command.
-
- Fixpoint defCommand (c: Command): (term unit unit) :=
-  match c with
-    | skip                => (@id unit)
-    | sequence c0 c1      => (defCommand c1) o (defCommand c0)
-    | assign i e0         => (update i) o (defArithExp e0)
-    | ifthenelse b c2 c3  => (copair (defCommand c2) (defCommand c3)) o (defBoolExp b)
-    | loops b c4          => (copair (loopdec o defCommand c4) (@id unit)) o (defBoolExp b)
-    | throwexc t0         => (throw unit t0)
-    | trycatch t1 c5 c6   => (@TRY_CATCH _ _ t1 (defCommand c5) (defCommand c6))
-  end.
-
- Notation "x '::=' a" := (assign x a) (at level 60).
- Notation "c1 ';;' c2" := (sequence c1 c2) (at level 65).
- Notation "'SKIP'" := (skip) (at level 60).
- Notation "'IFB' b 'THEN' t1 'ELSE' t2 'FI'" := (ifthenelse b t1 t2) (at level 60).
- Notation "'WHILE' b 'DO' c" := (loops b c) (at level 60).
- Notation " x '+++' y" := (add x y) (at level 60).
- Notation " x '***' y" := (multiply x y) (at level 60).
- Notation " x '>>' y" := (gtT x y) (at level 63).
- Notation " x '>>=' y" := (geT x y) (at level 63).
- Notation " x '<<' y" := (ltT x y) (at level 63).
- Notation " x '<<=' y" := (leT x y) (at level 63).
- Notation " x '===' y" := (eqT x y) (at level 63).
- Notation " x '&&&' y" := (andT x y) (at level 64).
- Notation " x '|||' y" := (orT x y) (at level 64).
- Notation "'THROW' en" := (throwexc en) (at level 60).
- Notation "'TRY' s0 'CATCH' e '=>' s1" := (trycatch e s0 s1) (at level 60).
- Notation "'{{' c '}}'" := (defCommand c) (at level 67).
- Notation "'``' c '``'" := (defBoolExp c) (at level 67).
-
- Parameter i j k: Loc.
- Parameter en: EName.
- Check {{ WHILE (constT ttrue) DO (i ::= (loc i +++ const 1)) }}.
- Check {{i ::= (loc j) ;; j ::= (const 5) ;; (k ::= (const 5) ;; SKIP)}}.
- Check (loc j) +++ (const 20) +++ (const 25) +++ (loc k).
- Check {{k ::= (loc i) ;; i ::= (loc j +++ const 20 +++ loc k +++ const 40) ;; k ::= (loc j)}}.
- Check {{i ::= (loc i +++ const 1)}}.
- Check (loc i +++ const 1).
- Check {{i ::= (loc i +++ const 1) ;; THROW en}}.
- Check {{THROW en ;; i ::= (loc i +++ const 1)}}.
- Check {{ i ::= (loc i +++ const 1);; THROW en }}.
- Check {{TRY (IFB (constT ttrue)
-               THEN (i ::= (loc i +++ const 1);;
-                     THROW en)
-              ELSE (SKIP)
-              FI)
-         CATCH en => (i ::= (const 10))}}.
-
- Eval simpl in k ::= (loc i) ;; i ::= (loc j +++ const 20 +++ loc k +++ const 40).
-
- Eval simpl in IFB (constF ffalse) 
-                 THEN (k ::= (loc i) ;; i ::= (loc j +++ const 20 +++ loc k +++ const 40))
-               ELSE (i ::= (loc j) ;; j ::= (const 5))
-               FI.
+  Module Export ConversionExp := IMP_to_COQ.Make(M).
 
  Lemma IMP_ex1: forall (x y: Loc) (p q: Z), x <> y ->
       {{x ::= (const p) ;; 
@@ -138,12 +36,12 @@ Module Make(Import M: Memory.T).
        {{IFB (constT ttrue) 
            THEN (m ::= const (-30)) 
          ELSE (SKIP)
-         FI}}
+         ENDIF}}
        ==
        {{IFB (constF ffalse) 
            THEN (SKIP) 
          ELSE (m ::= const (-30))
-         FI}}.
+         ENDIF}}.
  Proof.
  intros. simpl.
  transitivity(update m o constant (-30)) .
@@ -152,6 +50,7 @@ Module Make(Import M: Memory.T).
  apply strong_coproj_copi2_rwrw. apply strong_refl.
  Qed.
 
+
  Lemma IMP_ex3: forall (x: Loc) (p q: Z),
       {{x ::= (const p)  ;;
         x ::= (const q)}}
@@ -159,7 +58,7 @@ Module Make(Import M: Memory.T).
       {{x ::= (const q)}}.
  Proof.
      intros. simpl.
-     apply observation. intros. destruct(Loc_dec i0 x). rewrite e.
+     apply observation. intros. destruct(Loc_dec i x). rewrite e.
      transitivity(lookup x o update x o constant q o 
      (forget o constant p)).
      transitivity(id o constant q o update x o constant p).
@@ -183,22 +82,22 @@ Module Make(Import M: Memory.T).
      rewrite assoc. apply weak_subs. apply axiom_1.
      rewrite <- assoc. apply zero_weak_repl. auto.
      rewrite id_src. apply weak_refl.
-     transitivity(lookup i0 o forget o constant q o update x o constant p).
+     transitivity(lookup i o forget o constant q o update x o constant p).
      rewrite assoc. rewrite assoc. apply weak_subs. apply weak_subs.
      rewrite assoc. apply weak_subs. apply axiom_2. auto.
-     transitivity(lookup i0 o id o update x o constant p).
+     transitivity(lookup i o id o update x o constant p).
      apply weak_subs. apply weak_subs. apply strong_to_weak. 
      rewrite <- assoc. apply strong_repl. apply zero_weak_to_strong.
      auto. auto. apply weak_final_unique.
-     transitivity(lookup i0 o forget o constant p).
+     transitivity(lookup i o forget o constant p).
      apply weak_subs.
-     transitivity(lookup i0 o update x).
+     transitivity(lookup i o update x).
      apply weak_subs. rewrite id_src. apply weak_refl.
      apply axiom_2. auto.
-     transitivity(lookup i0 o id). apply strong_to_weak.
+     transitivity(lookup i o id). apply strong_to_weak.
      rewrite <- assoc. apply strong_repl. apply zero_weak_to_strong.
      auto. auto. apply weak_final_unique. apply weak_sym.
-     transitivity(lookup i0 o forget o constant q).
+     transitivity(lookup i o forget o constant q).
      rewrite assoc. apply weak_subs. apply axiom_2. auto.
      apply strong_to_weak. rewrite <- assoc. apply strong_repl.
      apply zero_weak_to_strong. auto. auto. apply weak_final_unique.  
@@ -222,7 +121,8 @@ Module Make(Import M: Memory.T).
      apply strong_to_weak. 
      transitivity(constant p o update x o constant p).
      rewrite assoc. rewrite assoc. apply strong_subs. apply strong_subs.
-     apply strong_proj_pi1_purepure. auto. auto.
+     apply one_weak_to_strong. auto. auto.
+     apply weak_proj_pi1_rorw. auto.
      remember commutation_lookup_constant.
      specialize(@commutation_lookup_constant x p). intros.
      apply strong_sym. apply H.
@@ -231,7 +131,7 @@ Module Make(Import M: Memory.T).
      apply strong_proj_pi2_rorw. auto. apply strong_sym.
      transitivity(constant q o update x o constant p).
      rewrite assoc. rewrite assoc. apply strong_subs. apply strong_subs.
-     apply strong_proj_pi2_purepure. auto. auto. apply strong_refl.
+     apply strong_proj_pi2_rorw. auto. apply strong_refl.
      transitivity((update x o constant (p+q) o (update x o constant p))).
      apply strong_subs. apply strong_repl. apply IMP_IntAdd.
      
@@ -257,7 +157,8 @@ Module Make(Import M: Memory.T).
      apply strong_to_weak. 
      transitivity(constant p o update x o constant p).
      rewrite assoc. rewrite assoc. apply strong_subs. apply strong_subs.
-     apply strong_proj_pi1_purepure. auto. auto.
+     apply one_weak_to_strong. auto. auto.
+     apply weak_proj_pi1_rorw. auto.
      remember commutation_lookup_constant.
      specialize(@commutation_lookup_constant x p). intros.
      apply strong_sym. apply H.
@@ -266,7 +167,7 @@ Module Make(Import M: Memory.T).
      apply strong_proj_pi2_rorw. auto. apply strong_sym.
      transitivity(constant q o update x o constant p).
      rewrite assoc. rewrite assoc. apply strong_subs. apply strong_subs.
-     apply strong_proj_pi2_purepure. auto. auto. apply strong_refl.
+     apply strong_proj_pi2_rorw. auto. apply strong_refl.
      transitivity((update x o constant (p*q) o (update x o constant p))).
      apply strong_subs. apply strong_repl. apply IMP_IntMult.
      
@@ -276,7 +177,8 @@ Module Make(Import M: Memory.T).
 
  Lemma IMP_ex6: forall (x: Loc),
       {{WHILE (constF ffalse) 
-          DO (x ::= (const 2)) ;; 
+          DO (x ::= (const 2))
+	ENDWHILE ;; 
         SKIP}}
       ==
       {{SKIP}}.
@@ -286,149 +188,12 @@ Module Make(Import M: Memory.T).
      apply strong_coproj_copi2_rwrw.
  Qed.
 
- Lemma pair_ex: forall (m: Loc) (c0 c1: Z),
-       gt o (pair (lookup m) (constant c1)) o update m o constant c0
-	~~
-       gt o (pair (constant c0) (constant c1)).  
- Proof.
-     intros. rewrite <- assoc. rewrite <- assoc.
-     apply zero_weak_repl. auto. apply unicity.
-     transitivity((lookup m) o (update m o constant c0)).
-     rewrite assoc. apply weak_subs.
-     apply weak_proj_pi1_rorw. auto.
-     transitivity(id o constant c0). rewrite assoc.
-     apply weak_subs. apply axiom_1. rewrite id_tgt.
-     apply weak_sym. apply weak_proj_pi1_rorw. auto.
-     transitivity(constant c1 o update m o constant c0).
-     rewrite assoc. rewrite assoc. apply weak_subs.
-     apply weak_subs. apply strong_to_weak.
-     apply strong_proj_pi2_rorw. auto.
-     transitivity(constant c1 o forget o constant c0).
-     apply weak_subs. apply zero_weak_repl.
-     auto. apply weak_final_unique.
-     transitivity(constant c1 o id). rewrite <- assoc.
-     apply zero_weak_repl. auto. apply weak_final_unique.
-     rewrite id_src. apply weak_sym. apply strong_to_weak.
-     apply strong_proj_pi2_rorw. auto.     
- Qed.
-
- Lemma pair_ex_2: forall (m n: Loc) (c0 c1: Z),
-       gt o (pair (lookup m) (constant c1)) o update m o constant c0 o update n o constant c1 
-	~~
-       gt o (pair (constant c0) (constant c1)).  
- Proof.
-     intros. rewrite <- assoc. rewrite <- assoc.
-     rewrite <- assoc. rewrite <- assoc.
-     apply zero_weak_repl. auto. apply unicity.
-     transitivity((lookup m) o (update m o constant c0) o (update n o constant c1)).
-     rewrite assoc. rewrite assoc. rewrite assoc. apply weak_subs.
-     rewrite <- assoc. apply weak_subs. apply weak_proj_pi1_rorw. auto.
-     transitivity(id o constant c0 o update n o constant c1).
-     rewrite assoc. apply weak_subs. apply weak_subs. 
-     rewrite assoc. apply weak_subs. apply axiom_1.
-     transitivity(id o constant c0 o forget o constant c1).
-     rewrite <- assoc. rewrite <- assoc. rewrite <- assoc.
-     rewrite <- assoc. apply zero_weak_repl. auto.
-     apply zero_weak_repl. auto. apply weak_final_unique.
-     transitivity(id o constant c0 o id). rewrite <- assoc.
-     apply zero_weak_repl. auto. apply weak_final_unique.
-     rewrite id_src. rewrite id_tgt. apply weak_sym. 
-     apply weak_proj_pi1_rorw. auto. 
-     transitivity(constant c1 o update m o constant c0 o update n o constant c1).
-     rewrite <- assoc.  rewrite <- assoc.  rewrite <- assoc. 
-     rewrite assoc. apply weak_subs. apply strong_to_weak.
-     apply strong_proj_pi2_rorw. auto.
-     transitivity((((constant c1 o forget) o constant c0) o update n) o constant c1).
-     apply weak_subs. apply weak_subs. apply weak_subs. 
-     apply zero_weak_repl. auto. apply weak_final_unique.
-     transitivity(constant c1 o forget o (constant c0) o forget o constant c1).
-     apply weak_subs. apply zero_weak_repl. auto. apply weak_final_unique.
-     transitivity((((constant c1 o forget) o constant c0) o id)).
-     rewrite <- assoc. apply zero_weak_repl. auto. apply weak_final_unique.
-     transitivity(constant c1 o id o id). apply weak_subs.
-     rewrite <- assoc. apply zero_weak_repl. auto. apply weak_final_unique.
-     rewrite id_src. rewrite id_src. apply weak_sym. apply strong_to_weak.
-     apply strong_proj_pi2_rorw. auto.     
- Qed.     
- 
-
- Lemma strong_pair: forall (m: Loc) (p q: Z),
-      (pair (lookup m) (constant q)) o update m o constant p
-      ==
-      (pair (constant p) (constant q)) o update m o constant p.
- Proof.
-      intros. apply strong_unicity.
-      transitivity(lookup m o update m o constant p).
-      rewrite assoc. apply weak_subs. rewrite assoc.
-      apply weak_subs. apply weak_proj_pi1_rorw. auto.
-      transitivity(id o constant p).
-      apply weak_subs. apply axiom_1. apply weak_sym.
-      transitivity(constant p o update m o constant p).
-      rewrite assoc. apply weak_subs. rewrite assoc.
-      apply weak_subs. apply weak_proj_pi1_rorw. auto.
-      rewrite id_tgt. setoid_rewrite <- id_src at 6.
-      rewrite <- assoc. apply zero_weak_repl. auto.
-      apply weak_final_unique.
-      transitivity(constant q o update m o constant p).
-      rewrite assoc. apply strong_subs. rewrite assoc.
-      apply strong_subs. apply strong_proj_pi2_rorw. auto.
-      apply strong_sym.
-      transitivity(constant q o update m o constant p).
-      rewrite assoc. apply strong_subs. rewrite assoc.
-      apply strong_subs. apply strong_proj_pi2_rorw. auto.
-      apply strong_refl.      
- Qed.
-
- (* Lemma strong_permpair: forall (m: Loc) (p q: Z),
-      (perm_pair (lookup m) (constant q)) o update m o constant p
-      ==
-      (perm_pair (constant p) (constant q)) o update m o constant p.
- Proof.
-      intros. apply strong_perm_unicity.
-      transitivity(lookup m o update m o constant p).
-      rewrite assoc. apply strong_subs. rewrite assoc.
-      apply strong_subs. apply strong_perm_proj_pi1_rwro. auto.
-      transitivity(constant p o update m o constant p).
-      specialize(@commutation_lookup_constant m p). intros.
-      apply H. apply strong_sym. rewrite assoc. apply strong_subs.
-      rewrite assoc. apply strong_subs.
-      apply strong_perm_proj_pi1_rwro. auto.
-      transitivity(constant q o update m o constant p).
-      rewrite assoc. apply weak_subs. rewrite assoc.
-      apply weak_subs. apply weak_perm_proj_pi2_rwro. auto.
-      apply weak_sym. rewrite assoc. apply weak_subs.
-      rewrite assoc. apply weak_subs. 
-      apply weak_perm_proj_pi2_rwro. auto.
- Qed. *)
-
- Lemma perm_strong_pair: forall (m: Loc) (p q: Z),
-      (pair (constant q) (lookup m)) o update m o constant p
-      ==
-      (pair (constant q) (constant p)) o update m o constant p.
- Proof.
-      intros. apply strong_unicity.
-      transitivity(constant q o update m o constant p).
-      rewrite assoc. apply weak_subs. rewrite assoc.
-      apply weak_subs. apply weak_proj_pi1_rorw. auto.
-      apply weak_sym. rewrite assoc. apply weak_subs.
-      rewrite assoc. apply weak_subs. 
-      apply weak_proj_pi1_rorw. auto.
-      transitivity(lookup m o update m o constant p).
-      rewrite assoc. apply strong_subs. rewrite assoc.
-      apply strong_subs. apply strong_proj_pi2_rorw. auto.
-      transitivity(constant p o update m o constant p).
-      specialize(@commutation_lookup_constant m p). intros.
-      apply H. apply strong_sym. rewrite assoc. apply strong_subs.
-      rewrite assoc. apply strong_subs.
-      apply strong_proj_pi2_rorw. auto.
- Qed.
-
  Lemma IMP_ex7: forall (x: Loc),
       {{x ::= (const 10) ;;
         IFB ((loc x) >> (const 5)) 
           THEN (x ::= (const 2)) 
         ELSE SKIP 
-        FI}}
+        ENDIF}}
       ==
       {{x ::= (const 2)}}.
  Proof.
@@ -455,7 +220,7 @@ Module Make(Import M: Memory.T).
         IFB ((loc x) >>= (const 5))
           THEN (x ::= (const 2)) 
         ELSE SKIP 
-        FI}}
+        ENDIF}}
       ==
       {{x ::= (const 2)}}.
  Proof.
@@ -482,13 +247,13 @@ Module Make(Import M: Memory.T).
         IFB ((loc x) >>= (const 0))
           THEN (SKIP) 
         ELSE (x ::= (loc x *** (const (-1)))) 
-        FI}}
+        ENDIF}}
       ==
       {{x ::= (const 10) ;;
         IFB ((loc x) <<= (const 0))
           THEN (x ::= (loc x *** (const (-1)))) 
         ELSE (SKIP) 
-        FI}}.
+        ENDIF}}.
  Proof.
     intros. unfold defCommand. unfold defBoolExp. 
     unfold defArithExp.
@@ -530,13 +295,13 @@ Module Make(Import M: Memory.T).
         IFB ((loc x) >>= (const 0)) 
           THEN (SKIP) 
         ELSE (x ::= (loc x *** (const (-1)))) 
-        FI}}
+        ENDIF}}
       ==
       {{x ::= (const (-10)) ;;
         IFB ((loc x) <<= (const 0)) 
           THEN (x ::= ( loc x *** (const (-1)))) 
         ELSE (SKIP) 
-        FI}}.
+        ENDIF}}.
  Proof.
     intros. unfold defCommand. unfold defBoolExp. 
     unfold defArithExp.
@@ -620,13 +385,13 @@ Module Make(Import M: Memory.T).
         IFB ((loc x) >>= (const 0)) 
           THEN (SKIP) 
         ELSE (x ::= (loc x *** (const (-1)))) 
-        FI}}
+        ENDIF}}
       ==
       {{x ::= (const 0) ;;
         IFB ((loc x) <<= (const 0))
           THEN (x ::= ( loc x *** (const (-1)))) 
         ELSE (SKIP) 
-        FI}}.
+        ENDIF}}.
  Proof.
     intros. unfold defCommand. unfold defBoolExp. 
     unfold defArithExp.
@@ -682,13 +447,13 @@ Module Make(Import M: Memory.T).
         IFB ((loc x) >>= (const 0)) 
           THEN (SKIP) 
         ELSE (x ::= ((const (-1)) *** loc x)) 
-        FI}}
+        ENDIF}}
       ==
       {{x ::= (const 0) ;;
         IFB ((loc x) <<= (const 0))
           THEN (x ::= ((const (-1)) *** loc x)) 
         ELSE (SKIP) 
-        FI}}.
+        ENDIF}}.
  Proof.
     intros. unfold defCommand. unfold defBoolExp. 
     unfold defArithExp.
@@ -769,14 +534,14 @@ Module Make(Import M: Memory.T).
         IFB ((loc x) >>= (loc y) *** (const 3))
           THEN (x ::= (loc y)) 
         ELSE (SKIP) 
-        FI}}
+        ENDIF}}
         ==
        {{x ::= (const 10) ;;
          y ::= (const 3) ;;
         IFB ((loc x) >>= (const 4) *** (loc y)) 
           THEN (SKIP) 
         ELSE (x ::= (loc y)) 
-        FI}}.
+        ENDIF}}.
  Proof.
     intros. unfold defCommand. unfold defBoolExp. 
     unfold defArithExp.
@@ -930,9 +695,9 @@ Module Make(Import M: Memory.T).
           THEN (IFB ((loc x) === (const 10))
                   THEN (x ::= (const 20))
                 ELSE (SKIP)
-                FI)
+                ENDIF)
         ELSE (x ::= (const 30)) 
-        FI}}
+        ENDIF}}
         ==
        {{x ::= (const 20)}}.
  Proof.
@@ -972,7 +737,8 @@ Module Make(Import M: Memory.T).
  Lemma IMP_ex15: forall (x: Loc),
 	{{x ::= (const 2) ;;
 	  WHILE ((loc x) << (const 11))
-	    DO (x ::= ((loc x) +++ (const 4)))}}
+	    DO (x ::= ((loc x) +++ (const 4)))
+	  ENDWHILE}}
 	==
 	{{x ::= (const 14)}}.
  Proof.
@@ -1099,64 +865,13 @@ Module Make(Import M: Memory.T).
     transitivity(id o (update x o constant 14)). apply strong_subs.
     apply strong_coproj_copi2_rwrw. rewrite id_tgt. apply strong_refl.
  Qed.
-       
 
- Lemma IMP_ex16: orB o (pair (le o (pair (@constant Z 80) (@constant Z 80)))
- (lt o (pair (@constant Z 180) (@constant Z 80))))
-       == 
-      ttrue.
- Proof.
-    apply IMP_IntOrT. left.
-    transitivity((le o pair (constant 80) (constant 80))).
-    apply strong_proj_pi1_purepure. auto. auto.
-    apply IMP_IntLeT. simpl. auto.
- Qed.
-
- Lemma IMP_ex17: orB o (pair (lt o (pair (@constant Z 80) (@constant Z 80)))
- (lt o (pair (@constant Z 180) (@constant Z 80))))
-       == 
-      ffalse.
- Proof.
-    apply IMP_IntOrF. 
-    transitivity((lt o pair (constant 80) (constant 80))).
-    apply strong_proj_pi1_purepure. auto. auto.
-    apply IMP_IntLtF. simpl. auto.
-    transitivity((lt o pair (constant 180) (constant 80))).
-    apply strong_proj_pi2_purepure. auto. auto.
-    apply IMP_IntLtF. simpl. auto.
- Qed.
-
- Lemma IMP_ex18: andB o (pair (le o (pair (@constant Z 80) (@constant Z 80)))
- (lt o (pair (@constant Z 180) (@constant Z 80))))
-       == 
-      ffalse.
- Proof.
-    apply IMP_IntAndF. right.
-    transitivity((lt o pair (constant 180) (constant 80))).
-    apply strong_proj_pi2_purepure. auto. auto.
-    apply IMP_IntLtF. simpl. auto.
- Qed.
-
- Lemma IMP_ex19: andB o (pair (le o (pair (@constant Z 80) (@constant Z 80)))
- (gt o (pair (@constant Z 180) (@constant Z 80))))
-       == 
-      ttrue.
- Proof.
-    apply IMP_IntAndT. 
-    transitivity((le o pair (constant 80) (constant 80))).
-    apply strong_proj_pi1_purepure. auto. auto.
-    apply IMP_IntLeT. simpl. auto.
-    transitivity((gt o pair (constant 180) (constant 80))).
-    apply strong_proj_pi2_purepure. auto. auto.
-    apply IMP_IntGtT. simpl. auto.
- Qed.
-
- Lemma IMP_ex20: forall (x: Loc),
+ Lemma IMP_ex16: forall (x: Loc),
        {{x ::= (const 50) ;;
          IFB ((loc x) << (const 70) &&& (loc x) >> (const 40))
            THEN (x ::= (const 10))
          ELSE (SKIP)
-         FI}}
+         ENDIF}}
        ==
        {{x ::= (const 10)}}.
  Proof.
@@ -1202,14 +917,56 @@ Module Make(Import M: Memory.T).
     ttrue o (update x o constant 50)).
     apply strong_sym. rewrite <- assoc. apply strong_repl.
     apply strong_subs. apply strong_sym. apply IMP_IntAndT.
-    apply strong_proj_pi1_purepure. apply is_ttrue. apply is_ttrue.
-    apply strong_proj_pi2_purepure. apply is_ttrue. apply is_ttrue.
-
+    apply one_weak_to_strong. auto. apply is_comp. auto.
+    apply is_pair. repeat apply is_pure_ro; apply is_ttrue.
+    repeat apply is_pure_ro; apply is_ttrue.
+    repeat apply is_pure_ro; apply is_ttrue. apply weak_proj_pi1_rorw. 
+    repeat apply is_pure_ro; apply is_ttrue.
+    apply strong_proj_pi2_rorw. repeat apply is_pure_ro; apply is_ttrue.
     transitivity((update x o constant 10) o (update x o constant 50)).
     apply strong_subs. apply strong_coproj_copi1_rwrw.
    
     specialize(@IMP_ex3 x 50 10). unfold defCommand. unfold defBoolExp. 
     unfold defArithExp. intros. apply H.    
+ Qed.
+
+ Lemma IMP_ex17: forall (x: Loc), forall (p: Z),
+         {{ IFB ((const p) << (const 0))
+           THEN (x ::= (const 100))
+         ELSE (x ::= (const p))
+         ENDIF}}
+         ==
+         {{ IFB ((const p) >>= (const 0))
+           THEN (x ::= (const p))
+         ELSE (x ::= (const 100))
+         ENDIF}}.
+ Proof.
+    intros. unfold defCommand. unfold defBoolExp. 
+    unfold defArithExp. induction p.
+    transitivity(copair (update x o constant 100) (update x o constant 0) o ffalse).
+    apply strong_repl. apply IMP_IntLtF. simpl. auto.
+    transitivity(update x o constant 0).
+    apply strong_coproj_copi2_rwrw. apply strong_sym.
+    transitivity(copair (update x o constant 0) (update x o constant 100) o ttrue).
+    apply strong_repl. apply IMP_IntGeT. simpl. auto.
+    transitivity(update x o constant 0).
+    apply strong_coproj_copi1_rwrw. apply strong_refl.
+    transitivity(copair (update x o constant 100) (update x o constant (Zpos p)) o ffalse).
+    apply strong_repl. apply IMP_IntLtF. simpl. auto.
+    transitivity(update x o constant (Zpos p)). apply strong_coproj_copi2_rwrw.
+    apply strong_sym.
+    transitivity(copair (update x o constant (Zpos p)) (update x o constant 100) o ttrue).
+    apply strong_repl. apply IMP_IntGeT. simpl. auto.
+    transitivity(update x o constant (Zpos p)). apply strong_coproj_copi1_rwrw.
+    apply strong_refl.
+    transitivity(copair (update x o constant 100) (update x o constant (Zneg p)) o ttrue).
+    apply strong_repl. apply IMP_IntLtT. simpl. auto.
+    transitivity(update x o constant 100). apply strong_coproj_copi1_rwrw.
+    apply strong_sym.
+    transitivity(copair (update x o constant (Zneg p)) (update x o constant 100) o ffalse).
+    apply strong_repl. apply IMP_IntGeF. simpl. auto.
+    transitivity(update x o constant 100). apply strong_coproj_copi2_rwrw.
+    apply strong_refl.
  Qed.
 
 End Make.
