Derived_Rules.v
@@ -1,19 +1,21 @@
 (**************************************************************************)
-(*  This is part of STATES, it is distributed under the terms of the      *)
-(*         GNU Lesser General Public License version 3                    *)
-(*              (see file LICENSE for more details)                       *)
+(*  This is part of IMP-STATES, it is distributed under the terms of the  *)
+(*              GNU Lesser General Public License version 3               *)
+(*                  (see file LICENSE for more details)                   *)
 (*                                                                        *)
-(*       Copyright 2013: Jean-Guillaume Dumas, Dominique Duval            *)
+(*       Copyright 2014: Jean-Guillaume Dumas, Dominique Duval            *)
 (*			 Burak Ekici, Damien Pous.                        *)
 (**************************************************************************)
 
 Require Import Relations Morphisms.
 Require Import Program.
-Require Memory Terms Decorations Axioms Derived_Terms Derived_Pairs Derived_Products.
+Require Memory Terms Decorations Derived_Terms Axioms.
 Set Implicit Arguments.
+Require Import ZArith.
+Open Scope Z_scope.
 
 Module Make(Import M: Memory.T).
-  Module Export Derived_RulesExp := Derived_Products.Make(M). 
+  Module Export Derived_RulesExp := Axioms.Make(M). 
 
 (* --- Derived Rules --- *)
 
@@ -38,7 +40,7 @@ Module Make(Import M: Memory.T).
      intros. assumption.
  Qed.
 
- Lemma E_1_1: forall X (f g: term unit X),
+Lemma E_1_1: forall X (f g: term unit X),
  is ro f -> is ro g -> f == g.
  Proof.
      intros. apply one_weak_to_strong.
@@ -117,71 +119,6 @@ Module Make(Import M: Memory.T).
      setoid_rewrite H0 at 1. apply weak_refl.     
  Qed.
 
- Lemma strong_unit_pi1__prod_forget: forall Y Z: Set,
-	 forget o pi1 == (@prod_forget Y Z).
- Proof.
-     intros. remember E_0_3. 
-     specialize(@E_0_3 _ _ forget prod_forget (@pi1 Y Z)).
-     intros. apply strong_sym. apply H. apply is_forget. 
-     apply is_prod_forget. apply is_pi1.
- Qed.
-
- Lemma strong_unit_pi2__prod_forget: forall (Y Z: Set),
- forget o pi2 == (@prod_forget Y Z).
- Proof.
-     intros. remember E_0_3. 
-     specialize(@E_0_3 _ _ forget prod_forget (@pi2 Y Z)).
-     intros. apply strong_sym. apply H. apply is_forget. 
-     apply is_prod_forget. apply is_pi2.
- Qed.
-
-Lemma strong_pi1_inv_pi1__id: forall Y: Set,
-pi1 o inv_pi1 == (@id Y).
- Proof.
-     intros. unfold inv_pi1.
-     remember strong_proj_pi1_purepure.
-     specialize(@strong_proj_pi1_purepure _ _ _
-     id (@forget Y)). 
-     intros. apply H. apply is_id. apply is_forget.
- Qed.
-
- Lemma strong_pi2_inv_pi1__unit: forall Y: Set,
- pi2 o inv_pi1 == (@forget Y).
- Proof.
-     intros. remember strong_proj_pi2_purepure.
-     specialize(@strong_proj_pi2_purepure _ _ _
-     id (@forget Y)). unfold inv_pi1. 
-     intros. apply H. apply is_id. apply is_forget.
- Qed.
-
- Lemma strong_pi1_permut__pi2: forall Y Z: Set,
- pi1 o permut == (@pi2 Y Z).
- Proof.
-     intros. unfold permut.
-     remember strong_proj_pi1_purepure.
-     specialize(@strong_proj_pi1_purepure _ _ _
-     (@pi2 Y Z) (pi1)).
-     intros. apply H. 
-     apply is_pi2. apply is_pi1. 
- Qed.
-
- Lemma strong_pi2_permut__pi1: forall Y Z: Set,
- pi2 o permut == (@pi1 Y Z).
- Proof.
-     intros. remember strong_proj_pi2_purepure.
-     specialize(@strong_proj_pi2_purepure _ _ _
-     (@pi2 Y Z) (pi1)). unfold permut. 
-     intros. apply H.
-     apply is_pi2. apply is_pi1. 
- Qed.
- 
- Lemma unicity_rect: forall X X' Y Y'(f g: term (Y/*/Y') (X/*/X')),
-   (pi1 o f ~~ pi1 o g) -> (pi2 o f ~~ pi2 o g) -> f ~~ g.
- Proof.
-     intros. remember unicity. apply unicity.
-     assumption. assumption.
- Qed.
- 
  Lemma strong_unicity: forall X Y Y'(f g: term (Y/*/Y') X),
    (pi1 o f ~~ pi1 o g) -> (pi2 o f == pi2 o g) -> f == g.
  Proof.
@@ -213,36 +150,6 @@ pi1 o inv_pi1 == (@id Y).
      assumption.
  Qed.
  
- Lemma strong_perm_unicity: forall X Y Y'(f g: term (Y'/*/Y) X),
-   (pi1 o f == pi1 o g) -> (pi2 o f ~~ pi2 o g) -> f == g.
- Proof.
-     intros.
-     remember comp_final_unique.
-     remember unicity.
-     apply comp_final_unique.
-     transitivity (forget o pi1 o f).
-     apply strong_subs.
-     apply E_0_1. apply is_forget. 
-     apply is_comp.
-     apply is_forget. apply is_pi1.
-     apply strong_sym.
-
-     transitivity (forget o pi1 o g).
-     apply strong_subs.
-     apply E_0_1. apply is_forget.
-     apply is_comp.
-     apply is_forget. apply is_pi1.
-     setoid_rewrite <- assoc at 1.
-     setoid_rewrite <- assoc at 1.
-     apply strong_repl.
-     apply strong_sym. assumption.
-
-     apply unicity.
-     apply strong_to_weak.
-     assumption.
-     assumption.
- Qed.
-
  Lemma strong_unicity_rect: forall X X' Y Y'(f g: term (Y/*/Y') (X/*/X')),
    (pi1 o f ~~ pi1 o g) -> (pi2 o f == pi2 o g) -> f == g.
  Proof.
@@ -251,62 +158,347 @@ pi1 o inv_pi1 == (@id Y).
      intros. apply H1. assumption. assumption.
  Qed.
 
- Lemma strong_perm_unicity_rect: forall X X' Y Y'(f g: term (Y/*/Y') (X/*/X')),
-   (pi1 o f == pi1 o g) -> (pi2 o f ~~ pi2 o g) -> f == g.
+ Lemma annihilation_update_lookup: forall i: Loc,
+ update i o lookup i == id. (* Prop: 2.1: All Cases *)
  Proof.
-     intros. remember strong_perm_unicity.
-     specialize (@strong_perm_unicity _ _ _ f g).
-     intros. apply H1. assumption. assumption.
+     intros. apply observation. intro k. intros.
+     destruct (Loc_dec i k). rewrite <- e.
+     (*Case k = i*)
+     rewrite assoc.
+     setoid_rewrite -> id_src. setoid_rewrite <- id_tgt at 6.
+     apply weak_subs. apply axiom_1.
+     (*Case k <> i*)
+     rewrite assoc.
+     transitivity (lookup k o forget o lookup i).
+     apply weak_subs. apply axiom_2. assumption.
+     apply strong_to_weak. rewrite <- assoc.
+     apply strong_repl. apply E_1_4. apply is_lookup.
  Qed.
 
- Lemma permuted_pair: forall X Y' Y (f1: term Y X) (f2: term Y' X), 
-  is ro f1 -> permut o perm_pair f2 f1 == pair f1 f2.
+ Lemma interaction_update_lookup: forall i: Loc,
+  lookup i o update i ~~ id. (* Prop: 2.4: All Cases *)
  Proof.
-     intros. remember strong_unicity.
-     specialize (@strong_unicity _ _ _ (permut o perm_pair f2 f1) (pair f1 f2)).
-     intros. apply H0.
-     transitivity (pi2 o perm_pair f2 f1).
-     rewrite -> assoc. apply weak_subs.
+     intros. apply axiom_1.
+ Qed.
 
-     remember weak_proj_pi1_rorw.
-     specialize(@weak_proj_pi1_rorw _ _ _
-     (@pi2 Y' Y) (pi1)).
-     intros. apply H1.
-     apply is_pure_ro. apply is_pi2.
- 
-     transitivity (f1).
-     apply weak_perm_proj_pi2_rwro. assumption.
-     apply weak_sym.
-     apply weak_proj_pi1_rorw. assumption.
-     
-     transitivity (pi1 o  perm_pair f2 f1).
-     rewrite assoc. apply strong_subs.
-     
-     remember strong_proj_pi2_rorw.
-     specialize(@strong_proj_pi2_rorw _ _ _
-     (@pi2 Y' Y) (pi1)). unfold permut. 
-     intros. apply H1.
-     apply is_pure_ro. apply is_pi2.
-     
-     transitivity (f2).
-     apply strong_perm_proj_pi1_rwro. assumption.
-
-     apply strong_sym.
-     apply strong_proj_pi2_rorw. assumption.
- Qed. 
-
- Lemma obs_local_global_2: forall X Y (f g : term Y X),
- (forall i: Loc, lookup i o forget o f ~~ lookup i o forget o g) ->  f ~~ g -> f == g.
+ Lemma commutation_lookup_constant: forall i: Loc, forall c: Z, 
+ lookup i o update i o (@constant Z c)
+ == 
+ (@constant Z c) o update i o (@constant Z c). (*Prop 2.8: All Cases*)
  Proof.
      intros. remember comp_final_unique.
-     specialize (@comp_final_unique _ _ f g).
-     intros. apply H1.
-     remember observation.
-     specialize (@observation _ (forget o f) (forget o g)).
-     intros. apply H2. 
-     setoid_rewrite assoc at 1. 
-     setoid_rewrite assoc at 1.
-     assumption. assumption.
+     specialize (@comp_final_unique _ _
+     ((lookup i o update i) o (@constant Z c)) (((@constant Z c) o update i) o (@constant Z c))).
+     intros. apply H.
+     (* Case 1: <> o f == <> o g *)
+     (*Step 1*)
+     transitivity (update i o (@constant Z c)).
+     setoid_rewrite -> assoc at 1.
+     apply strong_subs.
+     setoid_rewrite -> assoc at 1.
+     setoid_rewrite <- id_tgt at 6.
+     apply strong_subs.
+     remember E_1_4.
+     specialize (@E_1_4 _ (lookup i)).
+     intros. apply H0. apply is_lookup.
+     (*Step 2*)
+     apply strong_sym.
+     setoid_rewrite -> assoc at 1.
+     apply strong_subs.
+     setoid_rewrite <- id_tgt at 6.
+     setoid_rewrite -> assoc at 1.
+     apply strong_subs.
+     remember E_0_4.
+     specialize (@E_0_4 _ (@constant Z c)).
+     intros. apply H0. apply is_constant.
+     (* Case 2: f ~~ g *)
+     (*Step 1*)
+     transitivity ((@constant Z c)).
+     setoid_rewrite <- id_tgt at 6.
+     apply weak_subs. apply axiom_1.
+     (*Step 2*)
+     apply weak_sym.
+     setoid_rewrite <- id_src at 6.
+     setoid_rewrite <- assoc at 1.
+     apply zero_weak_repl. apply is_constant.
+     remember weak_final_unique.
+     specialize (@weak_final_unique _ (update i o (@constant Z c)) (id)).
+     intros. apply H0.
+ Qed.
+
+ Lemma commutation_update_x_update_y: forall {x y: Loc}, forall (n m: Z), x<>y -> 
+	(update y) o (@constant Z m) o (update x) o (@constant Z n) == 
+        (update x) o (@constant Z n) o (update y) o (@constant Z m).
+ Proof.
+    intros. apply observation. intros.
+    (* i = y *)
+    destruct (Loc_dec i y). rewrite e.
+    (*step 1*)
+    transitivity(id o (@constant Z m) o (update x) o (@constant Z n)).
+    rewrite assoc. apply weak_subs. rewrite assoc.
+    apply weak_subs. rewrite assoc.  apply weak_subs.
+    apply axiom_1.
+    (*step 2*)
+    transitivity ((@id Z) o (@constant Z m) o (@id (unit))).
+    rewrite <-assoc. rewrite <- assoc. rewrite <- assoc.
+    apply zero_weak_repl. apply is_id. apply zero_weak_repl.
+    apply is_constant. apply weak_final_unique.
+    apply weak_sym.
+    (*step 3*)
+    transitivity((lookup y) o forget o (@constant Z n) o (update y) o (@constant Z m)).
+    rewrite assoc; apply weak_subs. rewrite assoc; apply weak_subs.
+    rewrite assoc; apply weak_subs. apply axiom_2. assumption.
+    (*step 4*)
+    transitivity((lookup y) o (update y) o (@constant Z m)).
+    apply weak_subs; apply weak_subs. apply strong_to_weak.
+    remember E_0_3.
+    setoid_rewrite <- id_src at 6. rewrite <- assoc.
+    apply strong_repl. specialize(@E_0_3 _ _ forget id (@constant Z n)).
+    intros. apply strong_sym. apply H0. apply is_forget.
+    apply is_id. apply is_constant.
+    (*step 5*)
+    transitivity(id o (@constant Z m)).
+    apply weak_subs. apply axiom_1.
+    rewrite <- assoc. apply zero_weak_repl. auto.
+    setoid_rewrite <- id_src at 1. apply weak_refl.
+    (* i = x *)
+    destruct (Loc_dec i x). rewrite e.
+    (*step 1*)
+    transitivity((lookup x) o forget o (@constant Z m) o (update x) o (@constant Z n)).
+    rewrite assoc. apply weak_subs. rewrite assoc. apply weak_subs.
+    rewrite assoc. apply weak_subs. apply axiom_2.  auto.
+    (*step 2*)
+    transitivity((lookup x) o (update x) o (@constant Z n)).
+    apply weak_subs. apply weak_subs. apply strong_to_weak.
+    setoid_rewrite <- id_src at 6. rewrite <- assoc.
+    apply strong_repl. specialize(@E_0_3 _ _ forget id (@constant Z m)).
+    intros. apply strong_sym. apply H0. apply is_forget.
+    apply is_id. apply is_constant.    
+    (*step 3*)
+    transitivity(id o (@constant Z n)).
+    apply weak_subs. apply axiom_1.
+    apply weak_sym.
+    (*step 4*)
+    transitivity(id o (@constant Z n) o update y o (@constant Z m)).
+    rewrite assoc. apply weak_subs. rewrite assoc.
+    apply weak_subs. rewrite assoc.  apply weak_subs.
+    apply axiom_1.
+    (*step 5*)
+    transitivity ((@id Z) o (@constant Z n) o (@id (unit))).
+    rewrite <-assoc. rewrite <- assoc. rewrite <- assoc.
+    apply zero_weak_repl. apply is_id. apply zero_weak_repl.
+    apply is_constant. apply weak_final_unique.
+    apply weak_sym.
+    rewrite <- assoc. apply zero_weak_repl. auto.
+    setoid_rewrite <- id_src at 1. apply weak_refl.
+    (* i <> x and i <> y *)
+    (*step 1*)
+    transitivity((lookup i) o forget o (@constant Z m) o (update x) o (@constant Z n)).
+    rewrite assoc. apply weak_subs. rewrite assoc. apply weak_subs.
+    rewrite assoc. apply weak_subs. apply axiom_2. auto.
+    (*step 2*)
+    transitivity((lookup i) o (update x) o (@constant Z n)).
+    apply weak_subs. apply weak_subs. apply strong_to_weak.
+    setoid_rewrite <- id_src at 6. rewrite <- assoc.
+    apply strong_repl. specialize(@E_0_3 _ _ forget id (@constant Z m)).
+    intros. apply strong_sym. apply H0. apply is_forget.
+    apply is_id. apply is_constant.
+    (*step 3*)
+    transitivity(lookup i o forget o (@constant Z n)).
+    apply weak_subs. apply axiom_2. auto.
+    (*step 4*)
+    transitivity(lookup i o (@id (unit))).
+    apply strong_to_weak. rewrite <- assoc. apply strong_repl.
+    specialize(@E_0_3 _ _ forget id (@constant Z n)).
+    intros. apply strong_sym. apply H0. apply is_forget.
+    apply is_id. apply is_constant.
+    apply weak_sym.
+    (*step 5*)
+    transitivity((lookup i) o forget o (@constant Z n) o (update y) o (@constant Z m)).
+    rewrite assoc. apply weak_subs. rewrite assoc. apply weak_subs.
+    rewrite assoc. apply weak_subs. apply axiom_2.  auto.
+    (*step 6*)
+    transitivity((lookup i) o (update y) o (@constant Z m)).
+    apply weak_subs. apply weak_subs. apply strong_to_weak.
+    setoid_rewrite <- id_src at 6. rewrite <- assoc.
+    apply strong_repl. specialize(@E_0_3 _ _ forget id (@constant Z n)).
+    intros. apply strong_sym. apply H0. apply is_forget.
+    apply is_id. apply is_constant.
+    (*step 7*)
+    transitivity(lookup i o forget o (@constant Z m)).
+    apply weak_subs. apply axiom_2. auto.
+    apply strong_to_weak. rewrite <- assoc.
+    apply strong_repl. specialize(@E_0_3 _ _ forget id (@constant Z m)).
+    intros. apply strong_sym. apply H0. apply is_forget.
+    apply is_id. apply is_constant.
+ Qed. 
+
+
+ Lemma pair_ex: forall (m: Loc) (c0 c1: Z),
+       gt o (pair (lookup m) (constant c1)) o update m o constant c0
+	~~
+       gt o (pair (constant c0) (constant c1)).  
+ Proof.
+     intros. rewrite <- assoc. rewrite <- assoc.
+     apply zero_weak_repl. auto. apply unicity.
+     transitivity((lookup m) o (update m o constant c0)).
+     rewrite assoc. apply weak_subs.
+     apply weak_proj_pi1_rorw. auto.
+     transitivity(id o constant c0). rewrite assoc.
+     apply weak_subs. apply axiom_1. rewrite id_tgt.
+     apply weak_sym. apply weak_proj_pi1_rorw. auto.
+     transitivity(constant c1 o update m o constant c0).
+     rewrite assoc. rewrite assoc. apply weak_subs.
+     apply weak_subs. apply strong_to_weak.
+     apply strong_proj_pi2_rorw. auto.
+     transitivity(constant c1 o forget o constant c0).
+     apply weak_subs. apply zero_weak_repl.
+     auto. apply weak_final_unique.
+     transitivity(constant c1 o id). rewrite <- assoc.
+     apply zero_weak_repl. auto. apply weak_final_unique.
+     rewrite id_src. apply weak_sym. apply strong_to_weak.
+     apply strong_proj_pi2_rorw. auto.     
+ Qed.
+
+ Lemma pair_ex_2: forall (m n: Loc) (c0 c1: Z),
+       gt o (pair (lookup m) (constant c1)) o update m o constant c0 o update n o constant c1 
+	~~
+       gt o (pair (constant c0) (constant c1)).  
+ Proof.
+     intros. rewrite <- assoc. rewrite <- assoc.
+     rewrite <- assoc. rewrite <- assoc.
+     apply zero_weak_repl. auto. apply unicity.
+     transitivity((lookup m) o (update m o constant c0) o (update n o constant c1)).
+     rewrite assoc. rewrite assoc. rewrite assoc. apply weak_subs.
+     rewrite <- assoc. apply weak_subs. apply weak_proj_pi1_rorw. auto.
+     transitivity(id o constant c0 o update n o constant c1).
+     rewrite assoc. apply weak_subs. apply weak_subs. 
+     rewrite assoc. apply weak_subs. apply axiom_1.
+     transitivity(id o constant c0 o forget o constant c1).
+     rewrite <- assoc. rewrite <- assoc. rewrite <- assoc.
+     rewrite <- assoc. apply zero_weak_repl. auto.
+     apply zero_weak_repl. auto. apply weak_final_unique.
+     transitivity(id o constant c0 o id). rewrite <- assoc.
+     apply zero_weak_repl. auto. apply weak_final_unique.
+     rewrite id_src. rewrite id_tgt. apply weak_sym. 
+     apply weak_proj_pi1_rorw. auto. 
+     transitivity(constant c1 o update m o constant c0 o update n o constant c1).
+     rewrite <- assoc.  rewrite <- assoc.  rewrite <- assoc. 
+     rewrite assoc. apply weak_subs. apply strong_to_weak.
+     apply strong_proj_pi2_rorw. auto.
+     transitivity((((constant c1 o forget) o constant c0) o update n) o constant c1).
+     apply weak_subs. apply weak_subs. apply weak_subs. 
+     apply zero_weak_repl. auto. apply weak_final_unique.
+     transitivity(constant c1 o forget o (constant c0) o forget o constant c1).
+     apply weak_subs. apply zero_weak_repl. auto. apply weak_final_unique.
+     transitivity((((constant c1 o forget) o constant c0) o id)).
+     rewrite <- assoc. apply zero_weak_repl. auto. apply weak_final_unique.
+     transitivity(constant c1 o id o id). apply weak_subs.
+     rewrite <- assoc. apply zero_weak_repl. auto. apply weak_final_unique.
+     rewrite id_src. rewrite id_src. apply weak_sym. apply strong_to_weak.
+     apply strong_proj_pi2_rorw. auto.     
+ Qed.     
+ 
+
+ Lemma strong_pair: forall (m: Loc) (p q: Z),
+      (pair (lookup m) (constant q)) o update m o constant p
+      ==
+      (pair (constant p) (constant q)) o update m o constant p.
+ Proof.
+      intros. apply strong_unicity.
+      transitivity(lookup m o update m o constant p).
+      rewrite assoc. apply weak_subs. rewrite assoc.
+      apply weak_subs. apply weak_proj_pi1_rorw. auto.
+      transitivity(id o constant p).
+      apply weak_subs. apply axiom_1. apply weak_sym.
+      transitivity(constant p o update m o constant p).
+      rewrite assoc. apply weak_subs. rewrite assoc.
+      apply weak_subs. apply weak_proj_pi1_rorw. auto.
+      rewrite id_tgt. setoid_rewrite <- id_src at 6.
+      rewrite <- assoc. apply zero_weak_repl. auto.
+      apply weak_final_unique.
+      transitivity(constant q o update m o constant p).
+      rewrite assoc. apply strong_subs. rewrite assoc.
+      apply strong_subs. apply strong_proj_pi2_rorw. auto.
+      apply strong_sym.
+      transitivity(constant q o update m o constant p).
+      rewrite assoc. apply strong_subs. rewrite assoc.
+      apply strong_subs. apply strong_proj_pi2_rorw. auto.
+      apply strong_refl.      
+ Qed.
+
+ Lemma perm_strong_pair: forall (m: Loc) (p q: Z),
+      (pair (constant q) (lookup m)) o update m o constant p
+      ==
+      (pair (constant q) (constant p)) o update m o constant p.
+ Proof.
+      intros. apply strong_unicity.
+      transitivity(constant q o update m o constant p).
+      rewrite assoc. apply weak_subs. rewrite assoc.
+      apply weak_subs. apply weak_proj_pi1_rorw. auto.
+      apply weak_sym. rewrite assoc. apply weak_subs.
+      rewrite assoc. apply weak_subs. 
+      apply weak_proj_pi1_rorw. auto.
+      transitivity(lookup m o update m o constant p).
+      rewrite assoc. apply strong_subs. rewrite assoc.
+      apply strong_subs. apply strong_proj_pi2_rorw. auto.
+      transitivity(constant p o update m o constant p).
+      specialize(@commutation_lookup_constant m p). intros.
+      apply H. apply strong_sym. rewrite assoc. apply strong_subs.
+      rewrite assoc. apply strong_subs.
+      apply strong_proj_pi2_rorw. auto.
+ Qed.
+
+ Lemma or_ex1: orB o (pair (le o (pair (@constant Z 80) (@constant Z 80)))
+ (lt o (pair (@constant Z 180) (@constant Z 80))))
+       == 
+      ttrue.
+ Proof.
+    apply IMP_IntOrT. left.
+    transitivity((le o pair (constant 80) (constant 80))).
+    apply one_weak_to_strong. auto. apply is_comp. auto.
+    apply is_pair. auto. auto. auto.
+    apply weak_proj_pi1_rorw. auto.
+    apply IMP_IntLeT. simpl. auto.
+ Qed.
+
+ Lemma or_ex2: orB o (pair (lt o (pair (@constant Z 80) (@constant Z 80)))
+ (lt o (pair (@constant Z 180) (@constant Z 80))))
+       == 
+      ffalse.
+ Proof.
+    apply IMP_IntOrF. 
+    transitivity((lt o pair (constant 80) (constant 80))).
+    apply one_weak_to_strong. auto. apply is_comp. auto.
+    apply is_pair. auto. auto. auto.
+    apply weak_proj_pi1_rorw. auto. apply IMP_IntLtF. simpl. auto.
+    transitivity((lt o pair (constant 180) (constant 80))).
+    apply strong_proj_pi2_rorw. auto. apply IMP_IntLtF. simpl. auto.
+ Qed.
+
+ Lemma and_ex1: andB o (pair (le o (pair (@constant Z 80) (@constant Z 80)))
+ (lt o (pair (@constant Z 180) (@constant Z 80))))
+       == 
+      ffalse.
+ Proof.
+    apply IMP_IntAndF. right.
+    transitivity((lt o pair (constant 180) (constant 80))).
+    apply strong_proj_pi2_rorw. auto. apply IMP_IntLtF. simpl. auto.
+ Qed.
+
+ Lemma and_ex2: andB o (pair (le o (pair (@constant Z 80) (@constant Z 80)))
+ (gt o (pair (@constant Z 180) (@constant Z 80))))
+       == 
+      ttrue.
+ Proof.
+    apply IMP_IntAndT. 
+    transitivity((le o pair (constant 80) (constant 80))).
+    apply one_weak_to_strong. auto. apply is_comp. auto.
+    apply is_pair. auto. auto. auto.
+    apply weak_proj_pi1_rorw. auto.
+    apply IMP_IntLeT. simpl. auto.
+    transitivity((gt o pair (constant 180) (constant 80))).
+    apply strong_proj_pi2_rorw. auto. apply IMP_IntGtT. simpl. auto.
  Qed.
 
 (* -------------------- End of Derived Rules -------------------- *)
