IMP_to_COQ.v
@@ -1,0 +1,94 @@
+(**************************************************************************)
+(*  This is part of IMP-STATES, it is distributed under the terms of the  *)
+(*              GNU Lesser General Public License version 3               *)
+(*                  (see file LICENSE for more details)                   *)
+(*                                                                        *)
+(*       Copyright 2014: Jean-Guillaume Dumas, Dominique Duval            *)
+(*			 Burak Ekici, Damien Pous.                        *)
+(**************************************************************************)
+
+Require Import Relations Morphisms.
+Require Import Program.
+Require Memory Terms Decorations Derived_Terms Axioms Derived_Rules.
+Set Implicit Arguments.
+Require Import ZArith.
+Open Scope Z_scope.
+
+Module Make(Import M: Memory.T).
+  Module Export ConversionExp := Derived_Rules.Make(M).
+
+ Inductive ArithExp : Type :=
+    | const    : Z -> ArithExp
+    | loc      : Loc -> ArithExp
+    | add      : ArithExp -> ArithExp -> ArithExp
+    | multiply : ArithExp -> ArithExp -> ArithExp.
+
+ Fixpoint defArithExp (a: ArithExp) : term Z unit :=
+  match a with
+    | const n        => (@constant Z n)
+    | loc x          => (lookup x)
+    | add t1 t2      => plus o (pair (defArithExp t1) (defArithExp t2))
+    | multiply t3 t4 => mult o (pair (defArithExp t3) (defArithExp t4))
+  end.
+
+ Inductive BoolExp : Type :=
+    | constT  : term boolT unit -> BoolExp
+    | constF  : term boolT unit -> BoolExp
+    | gtT     : ArithExp -> ArithExp -> BoolExp
+    | geT     : ArithExp -> ArithExp -> BoolExp
+    | ltT     : ArithExp -> ArithExp -> BoolExp
+    | leT     : ArithExp -> ArithExp -> BoolExp
+    | eqT     : ArithExp -> ArithExp -> BoolExp
+    | andT    : BoolExp -> BoolExp -> BoolExp
+    | orT     : BoolExp -> BoolExp -> BoolExp.
+
+ Fixpoint defBoolExp (b: BoolExp) : term boolT unit :=
+  match b with
+    | constT ttrue  => ttrue
+    | constF ffalse => ffalse
+    | gtT a1 a2     => (gt o (pair (defArithExp a1) (defArithExp a2)))
+    | geT a1 a2     => (ge o (pair (defArithExp a1) (defArithExp a2)))
+    | ltT a1 a2     => (lt o (pair (defArithExp a1) (defArithExp a2)))
+    | leT a1 a2     => (le o (pair (defArithExp a1) (defArithExp a2)))
+    | eqT a1 a2     => (eq o (pair (defArithExp a1) (defArithExp a2)))
+    | andT b1 b2    => (andB o (pair (defBoolExp b1) (defBoolExp b2)))
+    | orT b3 b4     => (orB o (pair (defBoolExp b3) (defBoolExp b4)))
+  end.
+
+ Inductive Command : Type :=
+    | skip       : Command
+    | sequence   : Command -> Command -> Command
+    | assign     : Loc -> ArithExp -> Command 
+    | ifthenelse : BoolExp -> Command -> Command -> Command
+    | loops      : BoolExp -> Command -> Command.
+
+ Fixpoint defCommand (c: Command): (term unit unit) :=
+  match c with
+    | skip                => (@id unit)
+    | sequence c0 c1      => (defCommand c1) o (defCommand c0)
+    | assign i e0         => (update i) o (defArithExp e0)
+    | ifthenelse b c2 c3  => (copair (defCommand c2) (defCommand c3)) o (defBoolExp b)
+    | loops b c4          => (copair (loopdec o defCommand c4) (@id unit)) o (defBoolExp b)
+  end.
+
+ Notation "x '::=' a" := (assign x a) (at level 60).
+ Notation "c1 ';;' c2" := (sequence c1 c2) (at level 65).
+ Notation "'SKIP'" := (skip) (at level 60).
+ Notation "'IFB' b 'THEN' t1 'ELSE' t2 'ENDIF'" := (ifthenelse b t1 t2) (at level 60).
+ Notation "'WHILE' b 'DO' c 'ENDWHILE'" := (loops b c) (at level 60).
+ Notation " x '+++' y" := (add x y) (at level 60).
+ Notation " x '***' y" := (multiply x y) (at level 60).
+ Notation " x '>>' y" := (gtT x y) (at level 63).
+ Notation " x '>>=' y" := (geT x y) (at level 63).
+ Notation " x '<<' y" := (ltT x y) (at level 63).
+ Notation " x '<<=' y" := (leT x y) (at level 63).
+ Notation " x '===' y" := (eqT x y) (at level 63).
+ Notation " x '&&&' y" := (andT x y) (at level 64).
+ Notation " x '|||' y" := (orT x y) (at level 64).
+ Notation "'{{' c '}}'" := (defCommand c) (at level 67).
+ Notation "'``' c '``'" := (defBoolExp c) (at level 67).
+
+(* -------------------- End of IMP to COQ conversion -------------------- *)
+
+End Make.
+
